Test/Demo.lean
@@ -1,118 +1,72 @@
-/-
-Copyright (c) 2025 Lean FRO LLC. All rights reserved.
-Released under Apache 2.0 license as described in the file LICENSE.
-Authors: Sebastian Graf
--/
 import MPL
-import MPL.Experimental.Do
-
-namespace MPL.Test.Demo
-open MPL
+import MPL.Experimental
 
 set_option grind.warning false
 
--- Hoare triple specifications defined in terms of weakest precondition predicate transformers
+open MPL
 
-def AppState := Nat × Nat
+--
+-- Bird's eye view
+--
 
-def mkFreshNat [Monad m] [MonadStateOf AppState m] : m Nat := do
-  let n ← Prod.fst <$> get
-  modify (fun s => (s.1 + 1, s.2))
-  pure n
+abbrev fib_spec : Nat → Nat
+| 0 => 0
+| 1 => 1
+| n+2 => fib_spec n + fib_spec (n+1)
 
-private abbrev st : SVal (AppState::σs) (Nat × Nat) := fun s => SVal.pure s
-
-@[spec]
-theorem mkFreshNat_spec [Monad m] [WPMonad m sh] :
-  ⦃⌜(#st).1 = n ∧ (#st).2 = o⌝⦄
-  (mkFreshNat : StateT AppState m Nat)
-  ⦃⇓ r => ⌜r = n ∧ (#st).1 = n + 1 ∧ (#st).2 = o⌝⦄ := by
-  unfold mkFreshNat
-  mintro h ∀s
-  mwp
-  simp
-
-@[spec]
-theorem mkFreshNat_spec'' [Monad m] [WPMonad m sh] :
-  ⦃fun s => Q.1 s.1 (s.1+1,s.2)⦄
-  (mkFreshNat : StateT AppState m Nat)
-  ⦃Q⦄ := by
-  unfold mkFreshNat
-  mintro h ∀s
-  mwp
-
--- #print triple
--- #print WP.wp
--- #print PredTrans
-
-
-
-
-
-
-
-
-
-
-
-
-
-
-
--- wp_simp rules:
-
--- #check WP.bind_apply
--- #check StateT.get_apply
--- #check MonadStateOf.modify_apply
-
-
-
-
-
-
-
-
-
-
-
-
-
--- intrinsic verification
-
-def mkFreshNat' {m : Type → Type} [Monad m] : StateT AppState m Nat
-  forall {ps} [WPMonad m ps] (n o : Nat)
-  requires s => ⌜s.1 = n ∧ s.2 = o⌝
-  ensures r s => ⌜r = n ∧ s.1 = n + 1 ∧ s.2 = o⌝
+-- Extended `def` syntax:
+def fib_impl (n : Nat) : Idd Nat
+  ensures r => r = fib_spec n
 := do
-  let n ← Prod.fst <$> get
-  modify (fun s => (s.1 + 1, s.2))
+  if n = 0 then return 0
+  let mut a := 0
+  let mut b := 1
+  invariant xs => a = fib_spec xs.rpref.length ∧ b = fib_spec (xs.rpref.length + 1)
+  for _ in [1:n] do
+    let a' := a
+    a := b
+    b := a' + b
+  return b
+
+-- intrinsic, automated proof:
+#check fib_impl.spec
+
+theorem fib_correct {n} : (fib_impl n).run = fib_spec n := by
+  generalize h : (fib_impl n).run = x
+  apply Idd.by_wp h
+  apply fib_impl.spec n True.intro
+
+
+-- extrinsic, manual proof:
+theorem fib_triple : ⦃⌜True⌝⦄ fib_impl n ⦃⇓ r => r = fib_spec n⦄ := by
+  unfold fib_impl
+  dsimp
+  mintro _
+  if h : n = 0 then simp [h] else
+  simp only [h]
+  mwp
+  mspec Specs.forIn_list (⇓ (⟨a, b⟩, xs) => a = fib_spec xs.rpref.length ∧ b = fib_spec (xs.rpref.length + 1)) ?step
+  case step => dsimp; intros; mintro _; mwp; simp_all
+  simp_all [Nat.sub_one_add_one]
+
+--
+-- Compositional proofs using Hoare triple specifications
+--
+
+abbrev AppState := Nat
+
+def mkFreshNat : StateM AppState Nat
+  forall (n : Nat)
+  requires s => ⌜s = n⌝
+  ensures r s => ⌜r = n ∧ s = n + 1⌝
+:= do
+  let n ← get
+  set (n+1)
   pure n
 
--- #print mkFreshNat'.spec
+#check mkFreshNat.spec
 
-
-
-
-
-
-
-
-
-
-
-
-
-
-
-
-
-
-
-
-
--- compositional proofs using Hoare triple specifications
-
-def mkFreshPair : StateM AppState (Nat × Nat) := do
+noncomputable def mkFreshPair : StateM AppState (Nat × Nat) := do
   let a ← mkFreshNat
   let b ← mkFreshNat
   pure (a, b)
@@ -124,133 +78,266 @@ theorem mkFreshPair_spec :
   ⦃⇓ (a, b) => ⌜a ≠ b⌝⦄ := by
   unfold mkFreshPair
   mintro - ∀s
-  mspec mkFreshNat_spec
+  mspec mkFreshNat.spec
   mintro ∀s
   mcases h with ⌜h₁⌝
-  mspec mkFreshNat_spec
+  mspec mkFreshNat.spec
   mintro ∀s
   mcases h with ⌜h₂⌝
   simp_all [h₁, h₂]
 
--- eliminating a Hoare triple spec into the pure world
-
-theorem mkFreshPair_correct : ∀ s, let (a,b) := (mkFreshPair.run s).1; a ≠ b :=
-  fun s => mkFreshPair_spec s True.intro
 
 
+--
+-- Proof mode
+--
 
+abbrev M := StateT Nat (StateT Char (StateT Bool (StateT String Idd)))
+axiom op : Nat → M Nat
+noncomputable def prog (n : Nat) : M Nat := do
+  let a ← op n
+  let b ← op a
+  let c ← op b
+  return (a + b + c)
 
+axiom isValid : Nat → Char → Bool → String → Prop
 
+axiom op.spec {n} : ⦃isValid⦄ op n ⦃⇓r => ⌜r > 42⌝ ∧ isValid⦄
 
+theorem prog.spec : ⦃isValid⦄ prog n ⦃⇓r => ⌜r > 100⌝ ∧ isValid⦄ := by
+  -- This is an example for the (emulated) proof experience without a proof mode.
+  -- Note that after every application of a spec, we need to reintroduce all state variables.
+  unfold prog
+  unfold Triple
+  change ∀ a b c d, isValid a b c d → _
+  intro a b c d h
+  set_option trace.mpl.tactics.spec true in
+  mstart; mspec op.spec; mstop
+  intro a b c d ⟨hr₁, hvalid⟩
+  mstart; mspec op.spec; mstop
+  intro a b c d ⟨hr₂, hvalid⟩
+  mstart; mspec op.spec; mstop
+  intro a b c d ⟨hr₃, hvalid⟩
+  mstart; mspec; mstop
+  simp_all
+  omega
 
+theorem prog.spec' : ⦃isValid⦄ prog n ⦃⇓r => ⌜r > 100⌝ ∧ isValid⦄ := by
+  unfold prog
+  mintro h
+  mspec op.spec
+  mcases h with ⟨hr₁, h⟩
+  mspec op.spec
+  mcases h with ⟨hr₂, h⟩
+  mspec op.spec
+  mcases h with ⟨hr₃, h⟩
+  mspec
+  mrefine ⟨?_, h⟩
+  mpure_intro
+  omega
 
+--
+-- mspec
+--
 
+example [WP m ps] (x : m α)
+   (hspec : ⦃P⦄ x ⦃Q⦄)
+   (hpre : P' ⊢ₛ P)
+   (hpost : Q ⊢ₚ Q')
+   : P' ⊢ₛ wp⟦x⟧ Q' := by
+  mintro h
+  mspec hspec
+  case pre1 => exact hpre
+  case post => exact hpost
 
+example [WP m ps] (x : m α) (Q : α → Assertion ps)
+   (hspec : ⦃P⦄ x ⦃⇓ v => Q v⦄)
+   (hpre : P' ⊢ₛ P)
+   (hpost : ∀ v, Q v ⊢ₛ Q'.1 v)
+   : P' ⊢ₛ wp⟦x⟧ Q' := by
+  mintro h
+  mspec hspec
+  case pre1 => exact hpre
+  case post.success => exact hpost r
 
+#check Specs.forIn_list
 
+--
+-- Verification conditions
+--
 
-
-
-
--- loop invariants
-
--- #print Idd
--- #print Specs.forIn_list
--- #print List.Zipper
-
-def fib_impl (n : Nat) : Idd Nat := do
-  if n = 0 then return 0
-  let mut a := 0
-  let mut b := 1
-  for _ in [1:n] do
-    let a' := a
-    a := b
-    b := a' + b
-  return b
-
-@[reducible]
-def fib_spec : Nat → Nat
-| 0 => 0
-| 1 => 1
-| n+2 => fib_spec n + fib_spec (n+1)
-
-theorem fib_triple : ⦃True⦄ fib_impl n ⦃⇓ r => r = fib_spec n⦄ := by
+theorem fib_impl_vcs
+    (Q : Nat → PostCond Nat PostShape.pure)
+    (I : (n : Nat) → (_ : ¬n = 0) →
+      PostCond (MProd Nat Nat × List.Zipper [1:n].toList) PostShape.pure)
+    (ret : (Q 0).1 0)
+    (loop_pre : ∀ n (hn : ¬n = 0), (I n hn).1 (⟨0, 1⟩, List.Zipper.begin _))
+    (loop_post : ∀ n (hn : ¬n = 0) r, (I n hn).1 (r, List.Zipper.end _) ⊢ₛ (Q n).1 r.snd)
+    (loop_step : ∀ n (hn : ¬n = 0) r rpref x suff (h : [1:n].toList = rpref.reverse ++ x :: suff),
+                  (I n hn).1 (r, ⟨rpref, x::suff, by simp[h]⟩) ⊢ₛ (I n hn).1 (⟨r.2, r.1+r.2⟩, ⟨x::rpref, suff, by simp[h]⟩))
+    : wp⟦fib_impl n⟧ (Q n) := by
+  apply fib_impl.fun_cases n _ ?case1 ?case2
+  case case1 => unfold fib_impl; intro h; mstart; simp only [*, reduceIte]; mspec
+  case case2 =>
+  intro hn
   unfold fib_impl
-  mintro -
-  mwp
+  simp only [*, reduceIte]
+  mstart
+  mspec
+  mspec
+  mspec
+  case inv => exact I n hn
+  case pre1 => mpure_intro; apply_rules [loop_pre]
+  case post.success => mspec; mpure_intro; apply_rules [loop_post]
+  case step =>
+    intros;
+    mintro _;
+    mspec
+    mspec
+    mpure_intro
+    apply_rules [loop_step]
+
+
+
+
+
+
+-- Recall from above:
+theorem fib_triple' : ⦃⌜True⌝⦄ fib_impl n ⦃⇓ r => r = fib_spec n⦄ := by
+  unfold fib_impl
+  dsimp
+  mintro _
   if h : n = 0 then simp [h] else
-  simp only [h, reduceIte]
-  mspec Specs.forIn_list ?inv ?step
-  case inv => exact PostCond.total fun (⟨a, b⟩, xs) => a = fib_spec xs.rpref.length ∧ b = fib_spec (xs.rpref.length + 1)
-  case pre1 => simp_all
-  case step => intros; mintro _; mwp; simp_all
+  simp only [h]
+  mwp
+  mspec Specs.forIn_list (⇓ (⟨a, b⟩, xs) => a = fib_spec xs.rpref.length ∧ b = fib_spec (xs.rpref.length + 1)) ?step
+  case step => dsimp; intros; mintro _; mwp; simp_all
   simp_all [Nat.sub_one_add_one]
 
-theorem fib_correct {n} : (fib_impl n).run = fib_spec n := by
-  generalize h : (fib_impl n).run = x
-  apply Idd.by_wp h
-  apply fib_triple True.intro
+-- Now decompose:
 
--- intrisically:
+theorem fib_triple_vcs : ⦃⌜True⌝⦄ fib_impl n ⦃⇓ r => r = fib_spec n⦄ := by
+  intro _
+  apply fib_impl_vcs
+  case I => intro n hn; exact ⇓ (⟨a, b⟩, xs) =>
+    a = fib_spec xs.rpref.length ∧ b = fib_spec (xs.rpref.length + 1)
+  case ret => rfl
+  case loop_pre => simp
+  case loop_post => simp_all[Nat.sub_one_add_one]
+  case loop_step => simp_all
 
-def fib_impl' (n : Nat) : Idd Nat
-  ensures r => r = fib_spec n
-:= do
-  if n = 0 then return 0
-  let mut a := 0
-  let mut b := 1
-  assert => a = 0 ∧ b = 1
-  invariant xs => a = fib_spec xs.rpref.length ∧ b = fib_spec (xs.rpref.length + 1)
-  for _ in [1:n] do
-    let a' := a
-    a := b
-    b := a' + b
-  return b
+-- mvcgen gives us `fib_impl_vcs`. In practice, we don't bother extracting a theorem for it and
+-- use `mvcgen` directly:
 
--- #check fib_impl'.spec
+theorem fib_triple_vcs' : ⦃⌜True⌝⦄ fib_impl n ⦃⇓ r => r = fib_spec n⦄ := by
+  mvcgen [fib_impl]
+  case inv => exact ⇓ (⟨a, b⟩, xs) =>
+    a = fib_spec xs.rpref.length ∧ b = fib_spec (xs.rpref.length + 1)
+  all_goals simp_all [Nat.sub_one_add_one]
 
-
-
-
-
-
-
-
-
+theorem fib_impl_vcs'
+    (Q : Nat → PostCond Nat PostShape.pure)
+    (I : (n : Nat) → (_ : ¬n = 0) →
+      PostCond (MProd Nat Nat × List.Zipper [1:n].toList) PostShape.pure)
+    (ret : (Q 0).1 0)
+    (loop_pre : ∀ n (hn : ¬n = 0), (I n hn).1 (⟨0, 1⟩, List.Zipper.begin _))
+    (loop_post : ∀ n (hn : ¬n = 0) r, (I n hn).1 (r, List.Zipper.end _) ⊢ₛ (Q n).1 r.snd)
+    (loop_step : ∀ n (hn : ¬n = 0) r rpref x suff (h : [1:n].toList = rpref.reverse ++ x :: suff),
+                  (I n hn).1 (r, ⟨rpref, x::suff, by simp[h]⟩) ⊢ₛ (I n hn).1 (⟨r.2, r.1+r.2⟩, ⟨x::rpref, suff, by simp[h]⟩))
+    : wp⟦fib_impl n⟧ (Q n) := by
+  mvcgen [fib_impl]
+  case inv => apply_rules [I]
+  all_goals simp_all
 
 
 
 
 
 
--- exceptions, transformer stacks
 
-example :
-  ⦃fun s => s = 4⦄
-  (do
-    let mut x := 0
-    let s ← get
-    for i in [1:s] do -- i in [1,2,3,4], x = [0,1,3,6,10]
-      x := x + i
-      if x > 4 then throw 42
-    set 1
-    return x
-    : ExceptT Nat (StateT Nat Idd) Nat)
-  ⦃post⟨fun _ _ => False, fun e s => e = 42 ∧ s = 4⟩⦄ := by
-  mintro h ∀s
+
+
+
+
+
+
+
+
+
+
+
+--
+-- A bit more complex and realistic example:
+-- Serialization/deserialization of a file format.
+--
+
+structure File where
+  bytes : Array UInt8
+  pos : Fin (bytes.size + 1)
+
+inductive FileError where
+  | invalidPos
+  | invalidFormat
+  | eof
+
+abbrev FileM := EStateM FileError File
+
+def FileM.read (nbytes : Nat) : FileM (Vector UInt8 nbytes) := do
+  let f ← get
+  let mut ret := Vector.replicate nbytes default
+  let mut pos := f.pos
+  for h₁ : i in [:nbytes] do
+    if h₂ : pos < f.bytes.size then
+      ret := ret.set i f.bytes[pos]
+      pos := pos.succ.castLT (by simp[h₂])
+    else
+      throw FileError.eof
+  set { f with pos := pos }
+  return ret
+
+theorem range_elim : List.range' s n = xs ++ i :: ys → i = s + xs.length := by
+  intro h
+  induction xs generalizing s n
+  case nil => cases n <;> simp_all[List.range']
+  case cons head tail ih =>
+    cases n <;> simp[List.range'] at h
+    have := ih h.2
+    simp[ih h.2]
+    omega
+
+def canRead (n : Nat) (f : File) : Prop :=
+  f.pos + n ≤ f.bytes.size
+
+def hasRead {n : Nat} (v : Vector UInt8 n) (oldF newF : File) : Prop :=
+  oldF.bytes = newF.bytes ∧ oldF.pos + n = newF.pos  ∧ oldF.bytes.extract oldF.pos newF.pos = v.toArray
+
+theorem read_spec :
+  ⦃fun f' => canRead n f' ∧ f' = f⦄ FileM.read n ⦃⇓ v => hasRead v f⦄ := by
+  mintro h ∀f'
   mpure h
-  subst h
+  have ⟨hread, hfile⟩ := h
+  subst hfile
+  unfold FileM.read
   mwp
-  mspec (Specs.forIn_list post⟨fun (r, xs) s => r ≤ 4 ∧ s = 4 ∧ r + xs.suff.sum > 4, fun e s => e = 42 ∧ s = 4⟩ ?step)
+  mspec (Specs.forIn'_list ?inv ?step)
+  case inv => exact ⇓ (⟨pos, buf⟩, xs) =>
+    ⌜pos = f'.pos + xs.pref.length ∧ pos + xs.suff.length ≤ f'.bytes.size
+    ∧ f'.bytes.extract f'.pos pos = buf.toArray.take xs.pref.length⌝
+  case pre1 => intro hread; simp_all[canRead]; omega
   case step =>
-    intro b pref x suff h
-    mintro hinv ∀b'
+    intro ⟨pos, buf⟩ pref i hi suff hsuff
+    have := range_elim hsuff
+    simp at this
+    subst_vars
+    mintro ⌜hinv⌝
+    simp at hinv
     mwp
-    simp_all only [h, List.sum_cons, SVal.ite_app]
-    mpure hinv
-    mpure_intro
     split
-    · grind
-    · omega
-  simp only [List.sum_nil]
-  mintro ∀s; simp; omega -- grind in 4.17
+    · mpure_intro
+      simp +arith [hinv]
+      sorry -- pure proof about offset arithmetic and Array.extract
+    · simp_all
+      omega
+  case post.except.handle => simp
+  mintro ∀f
+  simp_all [hasRead]
