MPL/Experimental.lean
@@ -3,5 +3,4 @@ Copyright (c) 2025 Lean FRO LLC. All rights reserved.
 Released under Apache 2.0 license as described in the file LICENSE.
 Authors: Sebastian Graf
 -/
-import MPL.Experimental.Tactic
 import MPL.Experimental.Do
